almost done sim.v without UPD

src/axiomatic/SimRel.v
@@ -31,17 +31,235 @@ Hint Resolve gstep_wf gstep_inc coh_wf.
 
 Section Monotone.
 
-Definition monotone (mo : event -> event -> Prop) f :=
+Definition monotone (mo : relation event) f :=
   forall a b, mo a b -> Time.lt (f a) (f b).
 
-Lemma new_f acts sb rmw rf mo sc acts' sb' rmw' rf' mo' sc'
-  prev a (GSTEP: gstep acts sb rmw rf mo sc acts' sb' rmw' rf' mo' sc' prev a)
-  f (MON: monotone mo f): 
-  exists f', << F: forall b, In b acts -> f' b = f b >> /\
-             << MON: monotone mo' f' >> /\
-             << N_ZERO: Time.lt Time.bot (f' a) >>.
-Admitted.
+Definition monotone_acts acts (mo : relation event) f :=
+  forall a b, mo a b -> In a acts -> In b acts -> Time.lt (f a) (f b).
 
+
+Lemma no_imm_predecessor_simpl 
+      (mo : relation event) (IRR: irreflexive mo) (T: transitive mo) acts a
+      (NEG : ~
+      (exists prev,
+         In prev acts /\
+         mo prev a /\
+         (forall y : event, mo prev y -> mo y a -> In y acts -> False)))
+      prev (IN: In prev acts) (MO: mo prev a) : False. 
+Proof.
+  ins; destruct NEG; revert prev IN MO.
+  remember (length acts) as n; revert acts Heqn; induction n; ins.
+    by destruct acts; ins; desf.
+  destruct (classic (exists y, In y acts /\ mo y a /\ mo prev y)); desf;
+  [|by exists prev; splits; eauto].
+  apply in_split_perm in IN; desf.
+  rewrite IN in *; ins; desf; try (by exfalso; eauto).
+  edestruct IHn as [k N]; desc; eauto; exists k; splits; ins;
+  rewrite IN in *; ins; desf; eauto.
+Qed.
+
+Lemma no_imm_successor_simpl 
+      (mo : relation event) (IRR: irreflexive mo) (T: transitive mo) acts a
+      (NEG : ~
+      (exists next,
+         In next acts /\
+         mo a next /\
+         (forall y : event, mo a y -> mo y next -> In y acts -> False)))
+      next (IN: In next acts) (MO: mo a next) : False. 
+Proof.
+  ins; eapply no_imm_predecessor_simpl with (mo := fun x y => mo y x); eauto;
+  red; ins; desf; eauto 10.
+Qed.
+
+Lemma find_free_interval acts mo (IRR: irreflexive mo) (T: transitive mo) 
+      A (dom: A -> event -> Prop) 
+      (D : forall x y, mo x y -> exists l, dom l x /\ dom l y)
+      (DD : forall x l1 l2, dom l1 x -> dom l2 x -> l1 = l2)
+      (TOT: forall l, is_total (dom l) mo) a 
+  f_from f_to (MON: monotone_acts acts mo f_to) 
+  (NADJ: forall x (MOx: mo x a)
+                  (IMMx: forall z, mo x z -> mo z a -> In z acts -> False) 
+                y (MOy: mo a y)
+                  (IMMy: forall z, mo a z -> mo z y -> In z acts -> False), 
+     f_to x <> f_from y)
+  (NBOT: forall y (MO: mo a y) 
+                  (IMM: forall z, mo a z -> mo z y -> In z acts -> False), 
+            Time.bot <> f_from y)
+  (WF: forall l x (INx: In x acts) (Dx: dom l x), Time.lt (f_from x) (f_to x))
+  (NIN: ~ In a acts)
+  (DJ: forall l x (INx: In x acts) (Dx: dom l x) y (NEQ: x <> y)
+                  (INy: In y acts) (Dy: dom l y),
+         Interval.disjoint (f_from x, f_to x) (f_from y, f_to y)) : 
+  exists from' to',
+    Time.lt from' to' /\ 
+    (forall x, In x acts -> mo x a -> Time.le (f_to x) from') /\
+    (forall x, In x acts -> mo a x -> Time.le to' (f_from x)).
+Proof.
+  destruct (classic (exists prev, In prev acts /\ mo prev a /\
+                                  (forall y, mo prev y -> mo y a -> In y acts -> False))) 
+    as [P|P'];
+  [ desc; pose (from' := f_to prev) | pose (from' := Time.bot); 
+    assert (P := no_imm_predecessor_simpl IRR T acts a P'); clear P' ];
+  exists from'; 
+  (destruct (classic (exists next, In next acts /\ mo a next /\
+                                  (forall y, mo a y -> mo y next -> In y acts -> False))) 
+     as [Q|Q'];
+    [desc; exists (f_from next) |  exists (Time.incr from');
+     assert (Q := no_imm_successor_simpl IRR T acts a Q'); clear Q' ]); subst from'.
+
+  assert (K: Interval.disjoint (f_from prev, f_to prev) (f_from next, f_to next)).
+    destruct (D prev next); desc; eauto.
+    by eapply DJ; eauto; ins; desf; intro; desf; eauto.
+  exploit D; try exact P0; intro Dp; desc.
+  exploit D; try exact Q0; intro Dn; desc.
+  assert (l0 = l) by eauto; subst; clear Dp0.
+  splits; ins. 
+    red in K; destruct (Time.le_lt_dec (f_from next) (f_to prev)) as [LE|LT]; desf.
+    exfalso; rewrite Time.le_lteq in *; desf; eauto.
+    2: by eapply eq_sym, NADJ in LE; eauto.
+    exploit (MON prev next); ins; eauto.  
+    by eapply (K (f_to prev)); econs; ins; eauto; 
+       rewrite Time.le_lteq; eauto.
+  rewrite Time.le_lteq.
+  destruct (classic (x = prev)) as [|N]; desf; eauto.
+    destruct (D _ _ H0) as [l' ?]; desc.
+    eapply TOT in N; eauto; desf; eauto; try solve [exfalso; eauto].
+    exploit (DD a l l'); eauto; ins; desf.
+  rewrite Time.le_lteq.
+  destruct (classic (x = next)) as [|N]; desf; eauto.
+    destruct (D _ _ H0) as [l' ?]; desc.
+    eapply TOT in N; eauto; desf; eauto; try solve [exfalso; eauto];
+     exploit (DD a l l'); eauto; ins; desf.
+  destruct (TimeFacts.le_lt_dec (f_from x) (f_from next)); eauto.
+  exfalso; eapply DJ with (x := x) (y:= next) (x0 := f_to next); eauto; 
+    try (by intro; desf; eauto); econs; ins; eauto; try rewrite Time.le_lteq;
+    eauto using TimeFacts.le_lt_lt.
+
+  splits; ins; eauto using Time.incr_spec; try solve [exfalso; eauto].
+  rewrite Time.le_lteq.
+  destruct (classic (x = prev)) as [|N]; desf; eauto.
+    destruct (D _ _ P0) as [l ?], (D _ _ H0) as [l' ?]; desc.
+    eapply TOT in N; eauto; desf; eauto; try solve [exfalso; eauto].
+    by exploit (DD a l l'); eauto; ins; desf.
+
+  splits; ins; eauto using Time.bot_spec; try solve [exfalso; eauto].
+    by generalize (Time.bot_spec (f_from next)); rewrite Time.le_lteq; 
+       intro M; desf; eauto; eapply NBOT in M; ins.
+  rewrite Time.le_lteq.
+  destruct (classic (x = next)) as [|N]; desf; eauto.
+    destruct (D _ _ Q0) as [l ?], (D _ _ H0) as [l' ?]; desc.
+    eapply TOT in N; eauto; desf; eauto; try solve [exfalso; eauto];
+    exploit (DD a l l'); eauto; ins; desf.
+  destruct (TimeFacts.le_lt_dec (f_from x) (f_from next)); eauto.
+  exfalso; eapply DJ with (x := x) (y:= next) (x0 := f_to next); eauto; 
+    try (by intro; desf; eauto); econs; ins; eauto; try rewrite Time.le_lteq;
+    eauto using TimeFacts.le_lt_lt.
+
+  by splits; intros; eauto using Time.incr_spec; try solve [exfalso; eauto]. 
+Qed.
+
+
+Lemma find_free_interval2 acts mo (IRR: irreflexive mo) (T: transitive mo) 
+      A (dom: A -> event -> Prop) 
+      (D : forall x y, mo x y -> exists l, dom l x /\ dom l y)
+      (DD : forall x l1 l2, dom l1 x -> dom l2 x -> l1 = l2)
+      (TOT: forall l, is_total (dom l) mo) a 
+  f_from f_to (MON: monotone_acts acts mo f_to) 
+  (NADJ: forall x (MOx: mo x a)
+                  (IMMx: forall z, mo x z -> mo z a -> In z acts -> False) 
+                y (MOy: mo a y)
+                  (IMMy: forall z, mo a z -> mo z y -> In z acts -> False), 
+     f_to x <> f_from y)
+  (NBOT: forall y (MO: mo a y) 
+                  (IMM: forall z, mo a z -> mo z y -> In z acts -> False), 
+            Time.bot <> f_from y)
+  (WF: forall l x (INx: In x acts) (Dx: dom l x), Time.lt (f_from x) (f_to x))
+  (NIN: ~ In a acts)
+  (DJ: forall l x (INx: In x acts) (Dx: dom l x) y (NEQ: x <> y)
+                  (INy: In y acts) (Dy: dom l y),
+         Interval.disjoint (f_from x, f_to x) (f_from y, f_to y)) : 
+  exists from' to',
+    << WF': Time.lt from' to' >> /\ 
+    << PREV': forall x, In x acts -> mo x a -> Time.lt (f_to x) from' >> /\
+    << NEXT': forall x, In x acts -> mo a x -> Time.lt to' (f_from x) >> /\
+    << NBOT': Time.bot <> from' >>.
+Proof.
+  edestruct find_free_interval as (from & to & K); eauto; desc.
+  exists (Time.middle from to), (Time.middle (Time.middle from to) to).
+  splits; ins.
+  - by do 2 apply Time.middle_spec.
+  - by eapply TimeFacts.le_lt_lt; eauto; apply Time.middle_spec.
+  - by eapply TimeFacts.lt_le_lt; eauto; do 2 apply Time.middle_spec.
+  - destruct (Time.middle_spec from to); ins.
+    intro X; rewrite <- X in *.
+    eapply Time.lt_strorder; eauto using Time.bot_spec, TimeFacts.lt_le_lt.
+Qed.
+
+Lemma time_lt_trans x y z : Time.lt x y -> Time.lt y z -> Time.lt x z.
+Proof. eby etransitivity. Qed.
+
+Lemma new_f acts mo (IRR: irreflexive mo) (T: transitive mo) 
+      A (dom: A -> event -> Prop) 
+      (D : forall x y, mo x y -> exists l, dom l x /\ dom l y)
+      (DD : forall x l1 l2, dom l1 x -> dom l2 x -> l1 = l2)
+      (TOT: forall l, is_total (dom l) mo) a 
+      (ACT : forall x l, dom l x -> In x (a :: acts))
+  f_from f_to (MON: monotone_acts acts mo f_to) 
+  (NADJ: forall x (MOx: mo x a)
+                  (IMMx: forall z, mo x z -> mo z a -> In z acts -> False) 
+                y (MOy: mo a y)
+                  (IMMy: forall z, mo a z -> mo z y -> In z acts -> False), 
+     f_to x <> f_from y)
+  (NBOT: forall y (MO: mo a y) 
+                  (IMM: forall z, mo a z -> mo z y -> In z acts -> False), 
+            Time.bot <> f_from y)
+  (WF: forall l x (INx: In x acts) (Dx: dom l x), Time.lt (f_from x) (f_to x))
+  (NIN: ~ In a acts)
+  (DJ: forall l x (INx: In x acts) (Dx: dom l x) y (NEQ: x <> y)
+                  (INy: In y acts) (Dy: dom l y),
+         Interval.disjoint (f_from x, f_to x) (f_from y, f_to y)) : 
+  exists f_from' f_to', 
+    << F_FROM: forall b, In b acts -> f_from' b = f_from b >> /\
+    << F_TO: forall b, In b acts -> f_to' b = f_to b >> /\
+    << TWF: forall l x (Dx: dom l x), Time.lt (f_from' x) (f_to' x) >> /\
+    << MON': monotone mo f_to' >> /\
+    << DJ' : forall l x (Dx: dom l x) y (NEQ: x <> y) (Dy: dom l y),
+         Interval.disjoint (f_from' x, f_to' x) (f_from' y, f_to' y) >> /\ 
+    << NADJ_L: forall y, mo y a -> f_to' y <> f_from' a >> /\
+    << NADJ_R: forall y, mo a y -> f_to' a <> f_from' y >> /\
+    << NBOT': Time.bot <> f_from' a >>.
+Proof.
+  edestruct find_free_interval2 as (from' & to' & K); eauto; desc.
+  exists (upd f_from a from'), (upd f_to a to');
+  splits; simpls; rewrite ?upds; ins;
+    try solve [ins; desf; desf; rewrite ?upds, ?updo; ins; intro; desf; eauto].
+    exploit ACT; eauto; intro;
+    desf; desf; rewrite ?upds, ?updo; eauto; subst; try intro; desf; desf; 
+    solve [etransitivity; eauto | exfalso; eauto].
+
+    red; ins.
+    exploit D; eauto; intro M; desc; generalize M, M0; ins; apply ACT in M; apply ACT in M0;
+    desf; desf; rewrite ?upds, ?updo; eauto; subst; try intro; desf; desf;
+    try solve [etransitivity; eauto | exfalso; eauto].
+
+    ins; destruct (ACT _ _ Dx); desf; destruct (ACT _ _ Dy); desf;
+      rewrite ?upds, ?updo; eauto; subst; try intro; desf; desf;
+      eauto; ins; destruct LHS, RHS; ins; eauto;
+    eapply TOT in NEQ; eauto;
+    des; eapply Time.lt_strorder; 
+         eauto using time_lt_trans, TimeFacts.le_lt_lt, TimeFacts.lt_le_lt. 
+
+    ins; desf; rewrite updo; try intro; desf; desf; eauto.
+    exploit D; eauto; intro M; desc; apply ACT in M; desf; eauto.
+    eapply Time.lt_strorder, PREV'; eauto. 
+
+    ins; desf; rewrite updo; try intro; desf; desf; eauto.
+    exploit D; eauto; intro M; desc; apply ACT in M0; desf; eauto.
+    eapply Time.lt_strorder, NEXT'; eauto. 
+Qed.
+
+
+(*
 Lemma new_from (f: event -> Time.t) acts to (NZ: Time.lt Time.bot to) :
   exists from, 
     Time.lt from to /\ 
@@ -61,6 +279,7 @@ Proof.
   exists from; split; ins; desf; eauto.
   by exfalso; eapply Time.lt_strorder; etransitivity; eauto.
 Qed. 
+*)
 
 Lemma monotone_converse a b l f acts mo
   (INa: In a acts) (INb: In b acts) (WRITEa: is_write a) (WRITEb: is_write b)
@@ -108,58 +327,59 @@ Qed.
 
 Section Simulation.
 
-Variable f : event -> Time.t.
+Variables f_from f_to : event -> Time.t.
 
 Variable acts : list event.  
 Variables sb rmw rf mo sc : relation event.
 
 Definition sim_msg b  rel :=
-  << UR: forall l, max_value f (fun a => msg_rel urr acts sb rmw rf sc l a b) 
+  << UR: forall l, max_value f_to (fun a => msg_rel urr acts sb rmw rf sc l a b) 
                              (LocFun.find l rel.(Capability.ur)) >> /\
-  << RW: forall l, max_value f (fun a => msg_rel rwr acts sb rmw rf sc l a b) 
+  << RW: forall l, max_value f_to (fun a => msg_rel rwr acts sb rmw rf sc l a b) 
                              (LocFun.find l rel.(Capability.rw)) >> /\
-  << SC: forall l, max_value f (fun a => msg_rel scr acts sb rmw rf sc l a b) 
+  << SC: forall l, max_value f_to (fun a => msg_rel scr acts sb rmw rf sc l a b) 
                              (LocFun.find l rel.(Capability.sc)) >>.
 
 Definition sim_mem_helper b from v rel :=
   << VAL: Some v = (val b) >> /\
-  << FROM: Time.lt from (f b) >> /\ 
+  << FROM: Time.lt from (f_to b) >> /\ 
 (*   << FROMRMW: (forall a (RFRMW: (rf ;; rmw) a b), from = f a) >> /\ *)
   << SIMMSG: sim_msg b rel >>.
 
-Definition sim_mem mem:=
+Definition sim_mem mem :=
   forall l, 
     << DOM: forall b, (In b acts) /\ (is_write b) /\ (loc b = Some l) -> 
-                Memory.get l (f b) mem <> None >> /\
+                Memory.get l (f_to b) mem <> None >> /\
     << SIMCELL: forall to from v rel 
-                (CELL: Memory.get l to mem = Some (from, (Message.mk v rel))),
-                exists b, (In b acts) /\ (is_write b) /\ (loc b = Some l) /\ (f b = to) /\
-                (sim_mem_helper b from v rel) >> /\
+                (CELL: Memory.get l to mem = Some (from, Message.mk v rel)),
+                exists b, In b acts /\ is_write b /\ loc b = Some l 
+                          /\ f_from b = from /\ f_to b = to /\
+                          sim_mem_helper b from v rel >> /\
     << UPDATES: forall a b (RF_RMW: (rf ;; rmw) a b) (LOC: loc a = Some l),
-                exists m, Memory.get l (f b) mem = Some ((f a), m) >>.
+                exists m, Memory.get l (f_to b) mem = Some (f_to a, m) >>.
 
 Definition sim_rel rel i :=
-  << REL_UR: forall l' l, max_value f (t_rel urr acts sb rmw rf sc i l' l) 
+  << REL_UR: forall l' l, max_value f_to (t_rel urr acts sb rmw rf sc i l' l) 
     (LocFun.find l (LocFun.find l' rel).(Capability.ur)) >> /\
-  << REL_UR: forall l' l, max_value f (t_rel rwr acts sb rmw rf sc i l' l) 
+  << REL_UR: forall l' l, max_value f_to (t_rel rwr acts sb rmw rf sc i l' l) 
     (LocFun.find l (LocFun.find l' rel).(Capability.rw)) >> /\
-  << REL_UR: forall l' l, max_value f (t_rel scr acts sb rmw rf sc i l' l) 
+  << REL_UR: forall l' l, max_value f_to (t_rel scr acts sb rmw rf sc i l' l) 
     (LocFun.find l (LocFun.find l' rel).(Capability.sc)) >>.
 
 Definition sim_cur cur i :=
-  << CUR_UR: forall l, max_value f (t_cur urr acts sb rmw rf sc i l) 
+  << CUR_UR: forall l, max_value f_to (t_cur urr acts sb rmw rf sc i l) 
     (LocFun.find l cur.(Capability.ur)) >> /\
-  << CUR_RW: forall l, max_value f (t_cur rwr acts sb rmw rf sc i l) 
+  << CUR_RW: forall l, max_value f_to (t_cur rwr acts sb rmw rf sc i l) 
     (LocFun.find l cur.(Capability.rw)) >> /\
-  << CUR_SC: forall l, max_value f (t_cur scr acts sb rmw rf sc i l) 
+  << CUR_SC: forall l, max_value f_to (t_cur scr acts sb rmw rf sc i l) 
     (LocFun.find l cur.(Capability.sc)) >>.
 
 Definition sim_acq acq i :=
-  << ACQ_UR: forall l, max_value f (t_acq urr acts sb rmw rf sc i l) 
+  << ACQ_UR: forall l, max_value f_to (t_acq urr acts sb rmw rf sc i l) 
     (LocFun.find l acq.(Capability.ur)) >> /\
-  << ACQ_RW: forall l, max_value f (t_acq rwr acts sb rmw rf sc i l) 
+  << ACQ_RW: forall l, max_value f_to (t_acq rwr acts sb rmw rf sc i l) 
     (LocFun.find l acq.(Capability.rw)) >> /\
-  << ACQ_SC: forall l, max_value f (t_acq scr acts sb rmw rf sc i l) 
+  << ACQ_SC: forall l, max_value f_to (t_acq scr acts sb rmw rf sc i l) 
     (LocFun.find l acq.(Capability.sc)) >>.
 
 Definition sim_commit commit i :=
@@ -169,16 +389,16 @@ Definition sim_commit commit i :=
 
 End Simulation.
 
-Definition sim_time  (op_st: Configuration.t) (ax_st: Machine.configuration) f :=
-  << MONOTONE: monotone (mo ax_st) f >> /\  
+Definition sim_time  (op_st: Configuration.t) (ax_st: Machine.configuration) f_from f_to :=
+  << MONOTONE: monotone (mo ax_st) f_to >> /\  
   << SIM_COMMIT: forall i foo local
         (TID: IdentMap.find i (Configuration.threads op_st) = Some (foo, local)),
-        sim_commit f (acts ax_st) (sb ax_st) (rmw ax_st) (rf ax_st) (sc ax_st) 
+        sim_commit f_to (acts ax_st) (sb ax_st) (rmw ax_st) (rf ax_st) (sc ax_st) 
                    local.(Local.commit) (Some i) >> /\
-  << SIM_SC_MAP: forall l, max_value f (S_tm (acts ax_st) (sb ax_st) (rmw ax_st) 
+  << SIM_SC_MAP: forall l, max_value f_to (S_tm (acts ax_st) (sb ax_st) (rmw ax_st) 
                                              (rf ax_st) l) 
                                      (LocFun.find l (Configuration.sc op_st))  >> /\
-  << SIM_MEM: sim_mem f (acts ax_st) (sb ax_st) (rmw ax_st) (rf ax_st) (sc ax_st) 
+  << SIM_MEM: sim_mem f_from f_to (acts ax_st) (sb ax_st) (rmw ax_st) (rf ax_st) (sc ax_st) 
                       (Configuration.memory op_st) >>.
 
 Definition sim (op_st: Configuration.t) (ax_st: Machine.configuration) :=
@@ -189,7 +409,13 @@ Definition sim (op_st: Configuration.t) (ax_st: Machine.configuration) :=
         (TID: IdentMap.find i (Configuration.threads op_st) = Some (foo, local)),
          local.(Local.promises) = Memory.bot>> /\
   << STATES: ts ax_st = IdentMap.map fst (Configuration.threads op_st) >> /\
-  exists f, << TIME : sim_time op_st ax_st f >>. 
+  exists f_from f_to, 
+    << TIME : sim_time op_st ax_st f_from f_to >> /\
+    << SPACE : forall x y (MO: mo ax_st x y) (NRMW: ~ (rf ax_st ;; rmw ax_st) x y),
+                 f_to x <> f_from y >> /\
+    << BSPACE : forall y (INy: In y (acts ax_st)) (W: is_write y)
+                       (NRMW: ~ exists x, (rf ax_st ;; rmw ax_st) x y),
+                 Time.bot <> f_from y >>.
 
 Lemma find_mapD A B tid (f: A -> B) x y :
   IdentMap.find tid (IdentMap.map f x) = Some y ->
